HOL_To_IMP_Minus/Refinements/HOL_To_IMP_Minus_Primitives.thy
@@ -4,39 +4,46 @@ theory HOL_To_IMP_Minus_Primitives
     HOL_Nat_To_IMP_Minus.HOL_Nat_To_IMP_Tactics
 begin
 
-paragraph \<open>Equality\<close>
-
-locale HOL_To_HOL_Nat =
-  notes transport_eq_id.partial_equivalence_rel_equivalenceI[per_intro del]
-  and transport_eq_restrict_id.partial_equivalence_rel_equivalence[per_intro del]
+context HOL_To_HOL_Nat
 begin
+
+declare transport_eq_id.partial_equivalence_rel_equivalenceI[per_intro del]
+and transport_eq_restrict_id.partial_equivalence_rel_equivalence[per_intro del]
+
+paragraph \<open>Numerals\<close>
+
+text \<open>Natural number numerals are directly mapped to IMP constans and hence must not be compiled.\<close>
+lemma Rel_nat_numeral [Rel_nat]: "((=) ===> Rel_nat) (numeral :: _ \<Rightarrow> nat) (numeral :: _ \<Rightarrow> nat)"
+  unfolding Rel_nat_nat_eq_eq by auto
+
+paragraph \<open>Equality\<close>
 
 definition "eq_nat (n :: nat) m \<equiv> if (n - m) + (m - n) = 0 then True_nat else False_nat"
 
-lemma eq_nat_eq [HOL_To_IMP_finish_simps]: "eq_nat n m = natify (n = m)"
-  unfolding eq_nat_def natify_bool_def by simp
+lemma eq_nat_eq_False_nat_iff [HOL_To_IMP_finish_simps]: "eq_nat x y = False_nat \<longleftrightarrow> x \<noteq> y"
+ unfolding eq_nat_def by (auto simp: True_nat_ne_False_nat)
 
 lemma Rel_nat_eq_nat [Rel_nat]: "(Rel_nat ===> Rel_nat ===> Rel_nat) eq_nat (=)"
 proof (intro rel_funI)
   fix x x' and y y' :: 'a
   assume "Rel_nat x y" "Rel_nat x' y'"
   then show "Rel_nat (eq_nat x x') (y = y')"
-  by (cases "y = y'") (simp add: Rel_nat_iff_eq_natify compile_nat_type_def.Rep_inject eq_nat_eq)
+  by (cases "y = y'") (auto simp: Rel_nat_iff_eq_natify compile_nat_type_def.Rep_inject eq_nat_def
+    natify_True_eq natify_False_eq)
 qed
 
 end
 
-locale HOL_Nat_To_IMP_Minus =
-  (*remove simplification rules interfering with refinement proofs*)
-  notes neq0_conv[iff del, symmetric, iff] Nat.One_nat_def[simp del]
-  and de_Morgan_disj[simp del] de_Morgan_conj[simp del] not_imp[simp del] disj_not1[simp del]
+context HOL_Nat_To_IMP_Minus
 begin
 
-sublocale HTHN : HOL_To_HOL_Nat .
+(*remove simplification rules interfering with refinement proofs*)
+declare neq0_conv[iff del, symmetric, iff] Nat.One_nat_def[simp del]
+and de_Morgan_disj[simp del] de_Morgan_conj[simp del] not_imp[simp del] disj_not1[simp del]
 
-declaration \<open>K HOL_Nat_To_IMP_Tailcalls_Tactics.add_SIMPS_TO_if_assumption_loop\<close>
+unbundle tcom_syntax
 
-context includes com_syntax and no com'_syntax
+context includes com_syntax and no com'_syntax and no tcom_syntax
 begin
 
 definition [compiled_IMP_Minus_const_def]:
@@ -71,8 +78,6 @@ paragraph \<open>Addition and Subtraction\<close>
 context HOL_To_HOL_Nat
 begin
 
-sublocale HNTIM : HOL_Nat_To_IMP_Minus .
-
 lemma Rel_nat_add [Rel_nat]:
   "(Rel_nat ===> Rel_nat ===> Rel_nat) (+) ((+) :: nat \<Rightarrow> _)"
   by (auto simp: Rel_nat_nat_eq_eq)
@@ -86,7 +91,7 @@ end
 context HOL_Nat_To_IMP_Minus
 begin
 
-context includes com_syntax and no com'_syntax
+context includes com_syntax and no com'_syntax and no tcom_syntax
 begin
 
 definition [compiled_IMP_Minus_const_def]:
@@ -129,29 +134,29 @@ lemma mul_acc_nat_eq_mul_add: "mul_acc_nat x y z = x * y + z"
   by (induction x y z arbitrary: z rule: mul_acc_nat.induct)
   (auto simp: mul_acc_nat.simps mult_eq_if)
 
+case_of_simps mul_acc_nat_eq : mul_acc_nat.simps
+function_compile_nat mul_acc_nat_eq
+
 lemma mul_eq_mul_acc_nat_zero: "x * y = mul_acc_nat x y 0"
   using mul_acc_nat_eq_mul_add by simp
 
-lemma Rel_nat_mul [Rel_nat]:
-  "(Rel_nat ===> Rel_nat ===> Rel_nat) (*) ((*) :: nat \<Rightarrow> _)"
-  by (auto simp: Rel_nat_nat_eq_eq)
+function_compile_nat mul_eq_mul_acc_nat_zero
 
 end
 
 context HOL_Nat_To_IMP_Minus
 begin
 
-lemma case_nat_eq_if: "(case n of 0 \<Rightarrow> x | Suc x \<Rightarrow> f x) = (if n = 0 then x else f (n - 1))"
-  by (cases n type: nat) auto
+declare case_nat_eq_if[simp]
+and case_bool_nat_def[simp]
+and Rel_nat_selector_Suc[Rel_nat]
 
-case_of_simps mul_acc_nat_eq[simplified case_nat_eq_if] : HTHN.mul_acc_nat.simps
-compile_nat mul_acc_nat_eq basename mul_acc
+lemmas mul_acc_nat_nat_eq = HTHN.mul_acc_nat_nat_eq_unfolded[unfolded case_nat_eq_if]
+compile_nat mul_acc_nat_nat_eq
+HOL_To_IMP_Minus_correct HTHN.mul_acc_nat_nat by cook
 
-HOL_To_IMP_Minus_correct HTHN.mul_acc_nat by cook
-
-compile_nat HTHN.mul_eq_mul_acc_nat_zero basename mul
-
-HOL_To_IMP_Minus_correct Groups.times by cook
+compile_nat HTHN.times_nat_eq_unfolded
+HOL_To_IMP_Minus_correct HTHN.times_nat by cook
 
 end
 
@@ -160,22 +165,10 @@ paragraph \<open>Boolean Operators\<close>
 context HOL_Nat_To_IMP_Minus
 begin
 
-compile_nat True_nat_def basename true
-
-declare_compiled_const True
-  return_register "true.ret"
-  argument_registers
-  compiled "tailcall_to_IMP_Minus true_IMP_tailcall"
-
+compile_nat True_nat_def
 HOL_To_IMP_Minus_correct True_nat by cook
 
-compile_nat False_nat_def basename false
-
-declare_compiled_const False
-  return_register "false.ret"
-  argument_registers
-  compiled "tailcall_to_IMP_Minus false_IMP_tailcall"
-
+compile_nat False_nat_def
 HOL_To_IMP_Minus_correct False_nat by cook
 
 end
@@ -183,29 +176,17 @@ end
 context HOL_To_HOL_Nat
 begin
 
-definition "not_nat (n :: nat) \<equiv> eq_nat n False_nat"
+lemma not_iff_eq_False: "\<not>b \<longleftrightarrow> b = False" by simp
 
-lemma not_nat_eq [HOL_To_IMP_finish_simps]: "not_nat n = natify (n = False_nat)"
-  unfolding not_nat_def eq_nat_eq by simp
-
-lemma Rel_nat_not_nat [Rel_nat]:
-  "(Rel_nat ===> Rel_nat) not_nat Not"
-  unfolding not_nat_eq by (intro rel_funI)
-  (auto simp: Rel_nat_bool_iff natify_True_eq natify_False_eq True_nat_ne_False_nat)
+function_compile_nat not_iff_eq_False
 
 end
 
 context HOL_Nat_To_IMP_Minus
 begin
 
-compile_nat HTHN.not_nat_def basename not
-
-declare_compiled_const HOL.Not
-  return_register "not.ret"
-  argument_registers "not.args.n"
-  compiled "tailcall_to_IMP_Minus not_IMP_tailcall"
-
-HOL_To_IMP_Minus_correct HTHN.not_nat by cook
+compile_nat HTHN.Not_nat_eq_unfolded
+HOL_To_IMP_Minus_correct HTHN.Not_nat by cook
 
 end
 
@@ -217,29 +198,23 @@ begin
 lemma max_nat_eq_if: "max (x :: nat) y = (if x - y \<noteq> 0 then x else y)"
   by simp
 
-lemma Rel_nat_max [Rel_nat]:
-  "(Rel_nat ===> Rel_nat ===> Rel_nat) max (max :: nat \<Rightarrow> _)"
-  by (intro rel_funI) (auto simp: Rel_nat_nat_eq_eq)
+function_compile_nat max_nat_eq_if
 
 lemma min_nat_eq_if: "min (x :: nat) y = (if x - y \<noteq> 0 then y else x)"
   by simp
 
-lemma Rel_nat_min [Rel_nat]:
-  "(Rel_nat ===> Rel_nat ===> Rel_nat) min (min :: nat \<Rightarrow> _)"
-  by (intro rel_funI) (auto simp: Rel_nat_nat_eq_eq)
+function_compile_nat min_nat_eq_if
 
 end
 
 context HOL_Nat_To_IMP_Minus
 begin
 
-compile_nat HTHN.max_nat_eq_if basename max
+compile_nat HTHN.max_nat_eq_unfolded
+HOL_To_IMP_Minus_correct HTHN.max_nat by cook
 
-HOL_To_IMP_Minus_correct max by cook
-
-compile_nat HTHN.min_nat_eq_if basename min
-
-HOL_To_IMP_Minus_correct min by cook
+compile_nat HTHN.min_nat_eq_unfolded basename min
+HOL_To_IMP_Minus_correct HTHN.min_nat by cook
 
 end
 
@@ -248,47 +223,25 @@ paragraph \<open>More Boolean Operators\<close>
 context HOL_To_HOL_Nat
 begin
 
-definition "conj_nat (x :: nat) y \<equiv> min (min x y) True_nat"
+lemma conj_eq_if_then_else: "b1 \<and> b2 \<longleftrightarrow> (if b1 then if b2 then True else False else False)"
+  by auto
 
-lemma conj_nat_eq [HOL_To_IMP_finish_simps]: "conj_nat x y = natify (x \<noteq> False_nat \<and> y \<noteq> False_nat)"
-  unfolding conj_nat_def by (auto simp: natify_bool_def False_nat_eq_zero True_nat_def)
+function_compile_nat conj_eq_if_then_else
 
-lemma Rel_nat_conj_nat [Rel_nat]:
-  "(Rel_nat ===> Rel_nat ===> Rel_nat) conj_nat (\<and>)"
-  unfolding conj_nat_eq by (intro rel_funI)
-  (auto simp: Rel_nat_bool_iff natify_True_eq natify_False_eq True_nat_ne_False_nat)
+lemma disj_eq_if_then_else: "b1 \<or> b2 \<longleftrightarrow> (if b1 then True else if b2 then True else False)"
+  by auto
 
-definition "disj_nat (x :: nat) y \<equiv> min (max x y) True_nat"
-
-lemma disj_nat_eq [HOL_To_IMP_finish_simps]: "disj_nat x y = natify (x \<noteq> False_nat \<or> y \<noteq> False_nat)"
-  unfolding disj_nat_def by (auto simp: natify_bool_def False_nat_eq_zero True_nat_def)
-
-lemma Rel_nat_disj_nat [Rel_nat]:
-  "(Rel_nat ===> Rel_nat ===> Rel_nat) disj_nat (\<or>)"
-  unfolding disj_nat_eq by (intro rel_funI)
-  (auto simp: Rel_nat_bool_iff natify_True_eq natify_False_eq True_nat_ne_False_nat)
+function_compile_nat disj_eq_if_then_else
 
 end
 
 context HOL_Nat_To_IMP_Minus
 begin
 
-compile_nat HTHN.conj_nat_def basename conj
-
-declare_compiled_const conj
-  return_register "conj.ret"
-  argument_registers "conj.args.x" "conj.args.y"
-  compiled "tailcall_to_IMP_Minus conj_IMP_tailcall"
-
+compile_nat HTHN.conj_nat_eq_unfolded
 HOL_To_IMP_Minus_correct HTHN.conj_nat by cook
 
-compile_nat HTHN.disj_nat_def basename disj
-
-declare_compiled_const disj
-  return_register "disj.ret"
-  argument_registers "disj.args.x" "disj.args.y"
-  compiled "tailcall_to_IMP_Minus disj_IMP_tailcall"
-
+compile_nat HTHN.disj_nat_eq_unfolded
 HOL_To_IMP_Minus_correct HTHN.disj_nat by cook
 
 end
@@ -298,48 +251,24 @@ paragraph \<open>More Orders\<close>
 context HOL_To_HOL_Nat
 begin
 
-definition "le_nat (x :: nat) y \<equiv> eq_nat (x - y) 0"
+lemma le_nat_iff_sub_eq_zero: "(x :: nat) \<le> y \<longleftrightarrow> x - y = 0" by auto
 
-lemma le_nat_eq [HOL_To_IMP_finish_simps]: "le_nat x y = natify (x \<le> y)"
-  unfolding le_nat_def eq_nat_eq by simp
+function_compile_nat le_nat_iff_sub_eq_zero
 
-lemma Rel_nat_le_nat [Rel_nat]:
-  "(Rel_nat ===> Rel_nat ===> Rel_nat) le_nat ((\<le>) :: nat \<Rightarrow> _)"
-  by (intro rel_funI)
-  (auto simp: Rel_nat_nat_eq_eq Rel_nat_bool_iff le_nat_eq natify_True_eq natify_False_eq)
+lemma lt_nat_iff_le_and_ne: "(x :: nat) < y \<longleftrightarrow> x \<le> y \<and> x \<noteq> y" by auto
 
-definition "lt_nat (x :: nat) y \<equiv> conj_nat (le_nat x y) (not_nat (eq_nat x y))"
-
-lemma lt_nat_eq [HOL_To_IMP_finish_simps]: "lt_nat x y = natify (x < y)"
-  unfolding lt_nat_def by (auto simp: natify_bool_def le_nat_eq conj_nat_eq not_nat_eq eq_nat_eq)
-
-lemma Rel_nat_lt_nat [Rel_nat]:
-  "(Rel_nat ===> Rel_nat ===> Rel_nat) lt_nat ((<) :: nat \<Rightarrow> _)"
-  by (intro rel_funI)
-  (auto simp: Rel_nat_nat_eq_eq Rel_nat_bool_iff lt_nat_eq natify_True_eq natify_False_eq)
+function_compile_nat lt_nat_iff_le_and_ne
 
 end
 
 context HOL_Nat_To_IMP_Minus
 begin
 
-compile_nat HTHN.le_nat_def basename le
+compile_nat HTHN.less_eq_nat_eq_unfolded
+HOL_To_IMP_Minus_correct HTHN.less_eq_nat by cook
 
-declare_compiled_const "ord_class.less_eq"
-  return_register "le.ret"
-  argument_registers "le.args.x" "le.args.y"
-  compiled "tailcall_to_IMP_Minus le_IMP_tailcall"
-
-HOL_To_IMP_Minus_correct HTHN.le_nat by cook
-
-compile_nat HTHN.lt_nat_def basename lt
-
-declare_compiled_const "ord_class.less"
-  return_register "lt.ret"
-  argument_registers "lt.args.x" "lt.args.y"
-  compiled "tailcall_to_IMP_Minus lt_IMP_tailcall"
-
-HOL_To_IMP_Minus_correct HTHN.lt_nat by cook
+compile_nat HTHN.less_nat_eq_unfolded
+HOL_To_IMP_Minus_correct HTHN.less_nat by cook
 
 end
 
@@ -355,25 +284,23 @@ declare div_acc_nat.simps[simp del]
 lemma div_acc_nat_eq_div_add: "div_acc_nat x y z = x div y + z"
   by (induction x y z rule: div_acc_nat.induct) (auto simp: div_acc_nat.simps div_if)
 
+function_compile_nat div_acc_nat.simps
+
 lemma div_eq_div_acc_nat_zero: "x div y = div_acc_nat x y 0"
   using div_acc_nat_eq_div_add by simp
 
-lemma Rel_nat_div [Rel_nat]:
-  "(Rel_nat ===> Rel_nat ===> Rel_nat) Rings.divide (divide :: nat \<Rightarrow> _)"
-  by (auto simp: Rel_nat_nat_eq_eq div_acc_nat_eq_div_add)
+function_compile_nat div_eq_div_acc_nat_zero
 
 end
 
 context HOL_Nat_To_IMP_Minus
 begin
 
-compile_nat HTHN.div_acc_nat.simps basename div_acc
+compile_nat HTHN.div_acc_nat_nat_eq_unfolded
+HOL_To_IMP_Minus_correct HTHN.div_acc_nat_nat by cook
 
-HOL_To_IMP_Minus_correct HTHN.div_acc_nat by cook
-
-compile_nat HTHN.div_eq_div_acc_nat_zero basename div
-
-HOL_To_IMP_Minus_correct Rings.divide by cook
+compile_nat HTHN.divide_nat_eq_unfolded
+HOL_To_IMP_Minus_correct HTHN.divide_nat by cook
 
 end
 
@@ -390,8 +317,7 @@ declare_compiled_const Suc
   argument_registers "suc.args.x"
   compiled suc_IMP
 
-HOL_To_IMP_Minus_correct Suc
-  unfolding suc_IMP_def
+HOL_To_IMP_Minus_correct Suc unfolding suc_IMP_def
   by (fastforce intro: terminates_with_res_IMP_MinusI terminates_with_IMP_MinusI)
 
 end
@@ -399,74 +325,108 @@ end
 context HOL_To_HOL_Nat
 begin
 
+function_compile_nat triangle_def
+
 lemma pair_nat_eq_triangle_add: "pair_nat a b = triangle (a + b) + a"
   unfolding pair_nat_eq prod_encode_def by simp
 
-lemma Rel_nat_triangle [Rel_nat]: "(Rel_nat ===> Rel_nat) triangle triangle"
-  by (auto simp: Rel_nat_nat_eq_eq)
-lemma Rel_nat_pair_nat [Rel_nat]:
-  "(Rel_nat ===> Rel_nat ===> Rel_nat) pair_nat pair_nat"
-  by (auto simp: Rel_nat_nat_eq_eq)
+text \<open>We generate unconditional equations for all functions used in the construction of natural
+number datatypes. This way, one can directly compile native nat-datatype functions without
+an intermediate transfer step.\<close>
 
-fun fst_acc_nat :: "nat \<Rightarrow> nat \<Rightarrow> nat" where
-  "fst_acc_nat k m = (if m \<le> k then m else fst_acc_nat (Suc k) (m - Suc k))"
-fun snd_nat_acc :: "nat \<Rightarrow> nat \<Rightarrow> nat" where
-  "snd_nat_acc k m = (if m \<le> k then k - m else snd_nat_acc (Suc k) (m - Suc k))"
-declare fst_acc_nat.simps[simp del] and snd_nat_acc.simps[simp del]
+function_compile_nat pair_nat_eq_triangle_add
+declare pair_nat_related_transfer[Rel_nat del]
 
-lemma app_eq_app_prod_decode_acc_if_eq_if:
-  assumes "\<And>k m. f k m = (if m \<le> k then g (m, k - m) else f (Suc k) (m - Suc k))"
-  shows "f k m = g (prod_decode_aux k m)"
-proof (induction k m rule: prod_decode_aux.induct)
-  case (1 k m)
-  then show ?case by (cases "m \<le> k") (simp add: assms prod_decode_aux.simps)
+lemma pair_nat_eq_triangle_nat: "pair_nat a b = triangle_nat (a + b) + a"
+proof -
+  from pair_nat_related_transfer have "pair_nat_nat = pair_nat"
+    unfolding Rel_nat_nat_eq_eq by (simp add: rel_fun_eq)
+  with Rel_nat_nat_eq_eq pair_nat_nat_eq_unfolded show ?thesis by auto
 qed
 
-lemma fst_acc_nat_eq_fst_prod_decode_aux [simp]: "fst_acc_nat k m = fst (prod_decode_aux k m)"
-  by (fact
-    app_eq_app_prod_decode_acc_if_eq_if[where g = fst, simplified fst_conv, OF fst_acc_nat.simps])
-
-lemma snd_nat_acc_eq_snd_prod_decode_aux [simp]: "snd_nat_acc k m = snd (prod_decode_aux k m)"
-  by (fact
-    app_eq_app_prod_decode_acc_if_eq_if[where g = snd, simplified snd_conv, OF snd_nat_acc.simps])
-
-lemma fst_nat_eq_fst_acc_nat: "fst_nat m = fst_acc_nat 0 m"
-  unfolding fst_nat_eq unpair_nat_eq prod_decode_def
-  by (subst fst_acc_nat_eq_fst_prod_decode_aux) simp
-
-lemma Rel_nat_fst_nat [Rel_nat]: "(Rel_nat ===> Rel_nat) fst_nat fst_nat"
-  by (auto simp: Rel_nat_nat_eq_eq)
-
-lemma snd_nat_eq_snd_nat_acc: "snd_nat m = snd_nat_acc 0 m"
-  unfolding snd_nat_eq unpair_nat_eq prod_decode_def
-  by (subst snd_nat_acc_eq_snd_prod_decode_aux) simp
-
-lemma Rel_nat_snd_nat [Rel_nat]: "(Rel_nat ===> Rel_nat) snd_nat snd_nat"
-  by (auto simp: Rel_nat_nat_eq_eq)
+lemma Rel_nat_pair_nat [Rel_nat]: "(Rel_nat ===> Rel_nat ===> Rel_nat) pair_nat pair_nat"
+  unfolding Rel_nat_nat_eq_eq by (simp add: rel_fun_eq)
 
 end
 
 context HOL_Nat_To_IMP_Minus
 begin
 
-lemmas triangle_eq = triangle_def[unfolded Suc_eq_plus1]
-compile_nat triangle_eq
-HOL_To_IMP_Minus_correct triangle by cook
+compile_nat HTHN.triangle_nat_eq_unfolded
+HOL_To_IMP_Minus_correct HTHN.triangle_nat by cook
 
-compile_nat HTHN.pair_nat_eq_triangle_add
+compile_nat HTHN.pair_nat_eq_triangle_nat
 HOL_To_IMP_Minus_correct pair_nat by cook
 
-compile_nat HTHN.fst_acc_nat.simps
-HOL_To_IMP_Minus_correct HTHN.fst_acc_nat by cook
+end
 
-compile_nat HTHN.fst_nat_eq_fst_acc_nat
+context HOL_To_HOL_Nat
+begin
+
+fun fst_acc_nat :: "nat \<Rightarrow> nat \<Rightarrow> nat" where
+  "fst_acc_nat k m = (if m \<le> k then m else fst_acc_nat (Suc k) (m - Suc k))"
+fun snd_acc_nat :: "nat \<Rightarrow> nat \<Rightarrow> nat" where
+  "snd_acc_nat k m = (if m \<le> k then k - m else snd_acc_nat (Suc k) (m - Suc k))"
+declare fst_acc_nat.simps[simp del] and snd_acc_nat.simps[simp del]
+
+function_compile_nat fst_acc_nat.simps
+function_compile_nat snd_acc_nat.simps
+
+lemma app_eq_app_prod_decode_acc_if_eq_if:
+  assumes "\<And>k m. f k m = (if m \<le> k then g (m, k - m) else f (Suc k) (m - Suc k))"
+  shows "f k m = g (prod_decode_aux k m)"
+proof (induction k m rule: prod_decode_aux.induct)
+  case (1 k m)
+  then show ?case by (cases "m \<le> k") (simp_all add: assms prod_decode_aux.simps)
+qed
+
+lemma fst_acc_nat_eq_fst_prod_decode_aux: "fst_acc_nat k m = fst (prod_decode_aux k m)"
+  by (fact
+    app_eq_app_prod_decode_acc_if_eq_if[where g = fst, unfolded fst_conv, OF fst_acc_nat.simps])
+
+lemma snd_acc_nat_eq_snd_prod_decode_aux: "snd_acc_nat k m = snd (prod_decode_aux k m)"
+  by (fact
+    app_eq_app_prod_decode_acc_if_eq_if[where g = snd, unfolded snd_conv, OF snd_acc_nat.simps])
+
+lemma fst_nat_eq_fst_acc_nat: "fst_nat m = fst_acc_nat 0 m"
+  unfolding fst_nat_eq unpair_nat_eq prod_decode_def
+  by (subst fst_acc_nat_eq_fst_prod_decode_aux) simp
+
+lemma snd_nat_eq_snd_acc_nat: "snd_nat m = snd_acc_nat 0 m"
+  unfolding snd_nat_eq unpair_nat_eq prod_decode_def
+  by (subst snd_acc_nat_eq_snd_prod_decode_aux) simp
+
+function_compile_nat fst_nat_eq_fst_acc_nat
+declare fst_nat_related_transfer[Rel_nat del]
+
+lemma fst_nat_eq_fst_acc_nat_nat: "fst_nat n = fst_acc_nat_nat 0 n"
+proof -
+  from fst_nat_related_transfer have "fst_nat_nat = fst_nat"
+    unfolding Rel_nat_nat_eq_eq by (simp add: rel_fun_eq)
+  with Rel_nat_nat_eq_eq fst_nat_nat_eq_unfolded show ?thesis by auto
+qed
+
+lemma Rel_nat_fst_nat [Rel_nat]: "(Rel_nat ===> Rel_nat) fst_nat fst_nat"
+  unfolding Rel_nat_nat_eq_eq by (simp add: rel_fun_eq)
+
+function_compile_nat snd_nat_eq_snd_acc_nat
+
+end
+
+context HOL_Nat_To_IMP_Minus
+begin
+
+compile_nat HTHN.fst_acc_nat_nat_eq_unfolded
+HOL_To_IMP_Minus_correct HTHN.fst_acc_nat_nat by cook
+
+compile_nat HTHN.snd_acc_nat_nat_eq_unfolded
+HOL_To_IMP_Minus_correct HTHN.snd_acc_nat_nat by cook
+
+compile_nat HTHN.fst_nat_eq_fst_acc_nat_nat
 HOL_To_IMP_Minus_correct fst_nat by cook
 
-compile_nat HTHN.snd_nat_acc.simps
-HOL_To_IMP_Minus_correct HTHN.snd_nat_acc by cook
-
-compile_nat HTHN.snd_nat_eq_snd_nat_acc
-HOL_To_IMP_Minus_correct snd_nat by cook
+compile_nat HTHN.snd_nat_nat_eq_unfolded
+HOL_To_IMP_Minus_correct HTHN.snd_nat_nat by cook
 
 end
 
@@ -474,7 +434,7 @@ context HOL_To_HOL_Nat
 begin
 
 lemma fun_pow_eq: "(f^^n) x = (case n of 0 => x | Suc n => (f^^n) (f x))"
-  by (simp add: HOL_Nat_To_IMP_Minus.case_nat_eq_if)
+  by (simp add: case_nat_eq_if)
 
 lemma nat_selector_eq: "nat_selector nargs arg n =
   (let x = (snd_nat ^^ (arg + 1)) n in if arg + 1 < nargs then fst_nat x else x)"
@@ -483,24 +443,40 @@ lemma nat_selector_eq: "nat_selector nargs arg n =
 definition "fun_pow_snd_nat n \<equiv> snd_nat^^n"
 lemmas fun_pow_snd_nat_eq = fun_pow_eq[of _ "snd_nat", folded fun_pow_snd_nat_def]
 
+function_compile_nat fun_pow_snd_nat_eq
+
+lemmas nat_selector_eq_fun_pow_snd_nat = nat_selector_eq[folded fun_pow_snd_nat_def]
+function_compile_nat nat_selector_eq_fun_pow_snd_nat
+declare nat_selector_related_transfer[Rel_nat del]
+
+lemma nat_selector_eq_nat: "nat_selector nargs arg n =
+  (let x = fun_pow_snd_nat_nat (arg + 1) n in If_nat (less_nat (arg + 1) nargs) (fst_nat x) x)"
+proof -
+  from nat_selector_related_transfer have "nat_selector_nat = nat_selector"
+    unfolding Rel_nat_nat_eq_eq by (simp add: rel_fun_eq)
+  with Rel_nat_nat_eq_eq nat_selector_nat_eq_unfolded show ?thesis by auto
+qed
+
+lemma Rel_nat_nat_selector [Rel_nat]:
+  "(Rel_nat ===> Rel_nat ===> Rel_nat ===> Rel_nat) nat_selector nat_selector"
+  unfolding Rel_nat_nat_eq_eq by (simp add: rel_fun_eq)
+
 end
 
 context HOL_Nat_To_IMP_Minus
 begin
-lemmas fun_pow_snd_nat_eq = HTHN.fun_pow_snd_nat_eq[simplified case_nat_eq_if]
 
-lemma eq_sub_one_if_suc_eq: "Suc n = m \<Longrightarrow> n = m - 1" by simp
-
+lemmas fun_pow_snd_nat_eq = HTHN.fun_pow_snd_nat_nat_eq_unfolded[unfolded case_nat_eq_if]
 compile_nat fun_pow_snd_nat_eq
-HOL_To_IMP_Minus_correct HOL_To_HOL_Nat.fun_pow_snd_nat
-  supply eq_sub_one_if_suc_eq[simp]
+
+HOL_To_IMP_Minus_correct HTHN.fun_pow_snd_nat_nat
+  supply Rel_nat_selector_Suc[Rel_nat]
   apply (tactic \<open>HM.correct_if_IMP_tailcall_correct_tac HT.get_IMP_def @{context} 1\<close>)
-  by (induction "s ''fun_pow_snd_nat.args.n''" arbitrary: s rule: nat.induct)
+  by (induction y arbitrary: ya s rule: nat.induct)
   (tactic \<open>HT.start_run_finish_case_tac HT.get_IMP_def HT.get_imp_minus_correct
     HB.get_HOL_eqs @{context} 1\<close>)+
 
-lemmas nat_selector_eq = HTHN.nat_selector_eq[folded HTHN.fun_pow_snd_nat_def]
-compile_nat nat_selector_eq
+compile_nat HTHN.nat_selector_eq_nat
 HOL_To_IMP_Minus_correct nat_selector by cook
 
 end
