HOL_To_IMP_Minus/Refinements/HOL_To_IMP_Minus_IS_To_VC_List.thy
@@ -24,35 +24,27 @@ end
 context HOL_To_HOL_Nat
 begin
 
-lemma If_eq_case: "HOL.If = (\<lambda>b x y. (case b of True \<Rightarrow> x | False \<Rightarrow> y))"
-  by (intro ext) simp
-lemma is_vc_list_eq[unfolded If_eq_case]:
-    "is_vc_list x = (if list_card (concat (fst x)) < (snd x) then x else (fst x, list_card (concat (fst x)) - (snd x)))"
-  unfolding is_vc_list_def by (auto split: prod.split)
-function_compile_nat is_vc_list_eq
+lemmas is_vc_list_eq = is_vc_list_def[unfolded case_prod_beta, THEN meta_fun_cong]
+function_compile_nat is_vc_list_def[unfolded case_prod_beta]
 
 end
 
 context HOL_Nat_To_IMP_Minus
 begin
 
-lemmas is_vc_list_nat_eq = HTHN.is_vc_list_nat_eq_unfolded[simplified case_prod_nat_def case_bool_nat_def]
+lemmas is_vc_list_nat_eq = HTHN.is_vc_list_nat_eq_unfolded[unfolded case_prod_nat_def]
 compile_nat is_vc_list_nat_eq
-HOL_To_IMP_Minus_correct HOL_To_HOL_Nat.is_vc_list_nat by cook
+HOL_To_IMP_Minus_correct HOL_To_HOL_Nat.is_vc_list_nat by (cook mode = induction)
 
 lemma is_vc_list_IMP_Minus_correct:
   assumes "Rel_nat (s ''is_vc_list_nat.args.x'') x"
-  shows "terminates_with_res_IMP_Minus
-     (tailcall_to_IMP_Minus is_vc_list_nat_IMP_tailcall) s
-     ''is_vc_list_nat.ret''
-     (natify (is_vc_list x))"
+  shows "terminates_with_res_IMP_Minus (tailcall_to_IMP_Minus is_vc_list_nat_IMP_tailcall) s
+    ''is_vc_list_nat.ret'' (natify (is_vc_list x))"
 proof -
   have "HTHN.is_vc_list_nat TYPE('a) (s ''is_vc_list_nat.args.x'') = natify (is_vc_list x)"
-    using HOL_To_HOL_Nat.is_vc_list_nat_eq_unfolded[OF assms]
-      HOL_To_HOL_Nat.Rel_nat_is_vc_list_nat_unfolded[OF assms]
+    using HTHN.is_vc_list_nat_eq_unfolded[OF assms] HTHN.Rel_nat_is_vc_list_nat_unfolded[OF assms]
     by (simp add: Rel_nat_iff_eq_natify)
-  then show ?thesis
-    using is_vc_list_nat_IMP_Minus_correct[of s x, OF assms] by argo
+  then show ?thesis using is_vc_list_nat_IMP_Minus_correct[of s, OF assms] by simp
 qed
 
 end
