HOL_To_IMP_Minus/Refinements/HOL_To_IMP_Minus_Pairs.thy
@@ -11,6 +11,7 @@ function_compile_nat fst_def
 function_compile_nat snd_def
 
 definition "rpair y x \<equiv> (x, y)"
+
 function_compile_nat rpair_def
 
 end
@@ -18,14 +19,16 @@ end
 context HOL_Nat_To_IMP_Minus
 begin
 
+declare Rel_nat_selector_prod[Rel_nat]
+
 compile_nat Pair_nat_def
 HOL_To_IMP_Minus_correct Pair_nat by cook
 
-lemmas fst_nat_eq = HTHN.fst_nat_eq_unfolded[simplified case_prod_nat_def]
+lemmas fst_nat_eq = HTHN.fst_nat_eq_unfolded[unfolded case_prod_nat_def]
 compile_nat fst_nat_eq
 HOL_To_IMP_Minus_correct HOL_To_HOL_Nat.fst_nat by cook
 
-lemmas snd_nat_eq = HTHN.snd_nat_eq_unfolded[simplified case_prod_nat_def]
+lemmas snd_nat_eq = HTHN.snd_nat_eq_unfolded[unfolded case_prod_nat_def]
 compile_nat snd_nat_eq
 HOL_To_IMP_Minus_correct HOL_To_HOL_Nat.snd_nat by cook
 
